<?xml version="1.0"?>
<!DOCTYPE rdf:RDF [
     <!ENTITY sports   "http://www.bbc.co.uk/ontologies/sport/3.2.ttl" >
     <!ENTITY events   "http://motools.sourceforge.net/event/event.n3" >
	 <!ENTITY dc	   "http://purl.org/dc/elements/1.1/#" >
	 <!ENTITY foaf     "http://xmlns.com/foaf/0.1/#" >
	 <!ENTITY e-sports "http://www.eitel-lopez.org/e-sports#" >
	 <!ENTITY e-games  "http://www.eitel-lopez.org/e-games#" >
	 <!ENTITY e-teams  "http://www.eitel-lopez.org/e-teams#" >
	 <!ENTITY dbpedia  "http://dbpedia.org/resource/" >
     <!ENTITY owl      "http://www.w3.org/2002/07/owl#" >
     <!ENTITY xsd      "http://www.w3.org/2001/XMLSchema#" >
   ]>

<rdf:RDF
  xmlns              = "http://www.eitel-lopez.org/e-sports#"
  xmlns:e-sports     = "http://www.eitel-lopez.org/e-sports#"
  xml:base           = "http://www.eitel-lopez.org/e-sports#"
  xmlns:sports       = "http://www.bbc.co.uk/ontologies/sport/3.2.ttl"
  xmlns:events       = "http://motools.sourceforge.net/event/event.n3"
  xmlns:dc           = "http://purl.org/dc/elements/1.1/#"
  xmlns:foaf		 = "http://xmlns.com/foaf/0.1/#"
  xmlns:e-games		 = "http://www.eitel-lopez.org/e-games#"
  xmlns:e-teams  	 = "http://www.eitel-lopez.org/e-teams#"
  xmlns:geonames	 = "http://www.geonames.org/ontology/ontology_v3.1.rdf#"
  xmlns:dbpedia		 = "http://dbpedia.org/resource/"
  xmlns:owl          = "http://www.w3.org/2002/07/owl#"
  xmlns:rdf          = "http://www.w3.org/1999/02/22-rdf-syntax-ns#"
  xmlns:rdfs         = "http://www.w3.org/2000/01/rdf-schema#"
  xmlns:xsd          = "http://www.w3.org/2001/XMLSchema#">
  
  <owl:Ontology rdf:about="">9
    <rdfs:comment xml:lang="en">We present here an example of OWL ontology</rdfs:comment>
    <owl:imports rdf:resource="http://www.bbc.co.uk/ontologies/sport/3.2.ttl"/>
    <owl:imports rdf:resource="http://purl.org/dc/elements/1.1/#"/>
	<owl:imports rdf:resource="http://xmlns.com/foaf/0.1/#" />
	<owl:imports rdf:resource="http://motools.sourceforge.net/event/event.n3"/>
	<owl:imports rdf:resource="http://www.geonames.org/ontology/ontology_v3.1.rdf" />
    <rdfs:label>ESports Ontology</rdfs:label>
    <owl:versionInfo rdf:datatype="&xsd;float">1.00</owl:versionInfo>
  </owl:Ontology>
  
  <owl:Class rdf:ID="Organization">
    <rdfs:comment xml:lang="en">
      Entity responsible of the management and regualation of any event
    </rdfs:comment>
    <rdfs:label xml:lang="en">organization</rdfs:label>
    <rdfs:label xml:lang="fr">organization</rdfs:label>
  </owl:Class>
  
  <owl:Class rdf:ID="EOrganization">
    <rdfs:comment xml:lang="en">
      Management unit responsible the organization of any sports event
    </rdfs:comment>
    <rdfs:label xml:lang="en">e-sports organization</rdfs:label>
    <rdfs:label xml:lang="fr">organization d'e-sports</rdfs:label>
  </owl:Class>
  
  <owl:ObjectProperty rdf:about="isOrganizationOf">
    <rdfs:comment xml:lang="en">
      This property relates the Organizer unit with the Event, ESport, ...
    </rdfs:comment>
    <owl:inverseOf rdf:resource="#hasOrganization" /> 
    <rdfs:domain rdf:resource="#Organization" />
    <rdfs:label xml:lang="en">isOrganizationOf</rdfs:label>
    <rdfs:label xml:lang="fr">organizationDe</rdfs:label>
  </owl:ObjectProperty>
  
  <owl:ObjectProperty rdf:about="hasOrganization">
    <rdfs:comment xml:lang="en">
      This property relates an Organization with its ESports, ECompetitions, Events, ...
    </rdfs:comment>
    <owl:inverseOf rdf:resource="#isOrganizationOf" /> 
    <rdfs:range rdf:resource="#Organization" />
    <rdfs:label xml:lang="en">hasOrganization</rdfs:label>
    <rdfs:label xml:lang="fr">organizationDe</rdfs:label>
  </owl:ObjectProperty>
  
  <owl:Class rdf:ID="Hobby">
    <rdfs:comment xml:lang="en">
      Game, pastime or activity
    </rdfs:comment> 
    <rdfs:label xml:lang="en">hobby</rdfs:label>
    <rdfs:label xml:lang="fr">hobby</rdfs:label>
  </owl:Class>
  
  <owl:Class rdf:ID="ESport">
    <rdfs:comment xml:lang="en">
      eSports (also known as electronic sports, esports, e-sports, 
      competitive (video) gaming, professional (video) gaming, or 
  	  pro-gaming) can be defined as a form of sports where the primary 
  	  aspects of the sport are facilitated by video games
    </rdfs:comment>
    <rdfs:subClassOf rdf:resource="#Hobby" />
    <rdfs:seeAlso>
      <rdf:Description rdf:about="https://en.wikipedia.org/wiki/ESports">
       <dc:format>text</dc:format>
      </rdf:Description>
    </rdfs:seeAlso>
    <rdfs:label xml:lang="en">e-sport</rdfs:label>
    <rdfs:label xml:lang="fr">e-sport</rdfs:label>
  </owl:Class>
  
  <owl:ObjectProperty rdf:ID="derivedFrom">
    <rdf:type rdf:resource="&owl;FunctionalProperty" />
    <rdfs:domain rdf:resource="ESports" />
    <rdfs:range rdf:resource="VideoGame" />
	<owl:minCardinality rdf:datatype="&xsd;nonNegativeInteger">1</owl:minCardinality>
    <rdfs:label xml:lang="en">derived from</rdfs:label>
    <rdfs:label xml:lang="fr">viens de</rdfs:label>
  </owl:ObjectProperty>
  
  <owl:ObjectProperty rdf:about="similarESport">
    <rdfs:comment xml:lang="en">
      Builds a relationship of similarity among the sports
    </rdfs:comment>
    <rdf:type rdf:resource="&owl;SymmetricProperty"/>
    <rdfs:label xml:lang="en">similar ESport</rdfs:label>
    <rdfs:label xml:lang="fr">similar ESport</rdfs:label>
  </owl:ObjectProperty>
  
  <owl:ObjectProperty rdf:ID="hasName">
    <rdfs:label xml:lang="en">name</rdfs:label>
    <rdfs:label xml:lang="fr">nom</rdfs:label>
  </owl:ObjectProperty>
  
  <owl:ObjectProperty rdf:ID="hasWeb">
    <rdfs:label xml:lang="en">web</rdfs:label>
    <rdfs:label xml:lang="fr">web</rdfs:label>
  </owl:ObjectProperty>
  
  <owl:ObjectProperty rdf:ID="hasUri">
    <rdfs:label xml:lang="en">uri</rdfs:label>
    <rdfs:label xml:lang="fr">uri</rdfs:label>
  </owl:ObjectProperty>
  
  <owl:ObjectProperty rdf:ID="hasDescription">
    <rdfs:label xml:lang="en">description</rdfs:label>
    <rdfs:label xml:lang="fr">description</rdfs:label>
  </owl:ObjectProperty>
  
  <owl:Class rdf:ID="Videogame">
    <rdfs:comment xml:lang="en">
      A videogame is an electronic game that involves human interaction with 
  	a user interface to generate visual feedback on a video device such as 
  	a TV screen or computer monitor
    </rdfs:comment>
    <rdfs:subClassOf rdf:resource="#Hobby" />
    <rdfs:seeAlso>
      <rdf:Description rdf:about="https://en.wikipedia.org/wiki/Video_game">
       <dc:format>text</dc:format>
      </rdf:Description>
    </rdfs:seeAlso>
    <rdfs:label xml:lang="en">videogame</rdfs:label>
    <rdfs:label xml:lang="fr">jéu vidéo</rdfs:label>
  </owl:Class>
  
  <owl:ObjectProperty rdf:ID="basedOn">
    <rdfs:comment xml:lang="en">
      Relates Videogames and ESports
    </rdfs:comment>
    <rdf:type rdf:resource="&owl;FunctionalProperty" />
    <rdfs:domain rdf:resource="Videogame" />
    <rdfs:range rdf:resource="ESports" />
    <rdfs:label xml:lang="en">based on</rdfs:label>
    <rdfs:label xml:lang="fr">basé sur</rdfs:label>
  </owl:ObjectProperty>
  
  <owl:Class rdf:ID="VideoConsole">
    <rdfs:comment xml:lang="en">
      A video game console is a device that outputs a video signal or visual 
  	image to display a video game
    </rdfs:comment>
    <rdfs:seeAlso>
      <rdf:Description rdf:about="https://en.wikipedia.org/wiki/Video_game_console">
       <dc:format>text</dc:format>
      </rdf:Description>
    </rdfs:seeAlso>
    <rdfs:label xml:lang="en">video console station</rdfs:label>
    <rdfs:label xml:lang="fr">console de jéu vidéo</rdfs:label>
  </owl:Class>
  
  <owl:ObjectProperty rdf:ID="hasWon">
    <rdfs:comment xml:lang="en">
      Property that gathers victories
    </rdfs:comment>
    <rdfs:label xml:lang="en">has won</rdfs:label>
    <rdfs:label xml:lang="fr">reussir</rdfs:label>
  </owl:ObjectProperty>
  
  <owl:ObjectProperty rdf:ID="playInConsole">
    <rdfs:comment xml:lang="en">
      Describes the platform in which the game is played
    </rdfs:comment>
    <rdf:type rdf:resource="&owl;FunctionalProperty" />
    <rdfs:domain rdf:resource="Videogame" />
    <rdfs:range rdf:resource="VideoConsole" />
    <rdfs:label xml:lang="en">play in console</rdfs:label>
    <rdfs:label xml:lang="fr">basé sur</rdfs:label>
  </owl:ObjectProperty>
  
  <owl:Class rdf:about="Event">
    <rdfs:subClassOf rdf:resource="&events;Event"/>
    <rdfs:subClassOf>
      <owl:Restriction>
        <owl:onProperty rdf:resource="&events;Place" />
        <owl:minCardinality rdf:datatype="&xsd;nonNegativeInteger">1</owl:minCardinality>
      </owl:Restriction>
    </rdfs:subClassOf>
  </owl:Class>
  
  <owl:ObjectProperty rdf:about="isEventOf">
    <rdfs:comment xml:lang="en">
      This property relates the Events with the ECompetitions
    </rdfs:comment>
    <owl:inverseOf rdf:resource="#hasEvent" /> 
    <rdfs:domain rdf:resource="#Event" />
    <rdfs:range rdf:resource="#ECompetition" />
    <rdfs:label xml:lang="en">isEventOf</rdfs:label>
    <rdfs:label xml:lang="fr">eventement de</rdfs:label>
  </owl:ObjectProperty>
  
  <owl:ObjectProperty rdf:about="hasEvent">
    <rdfs:comment xml:lang="en">
      This property relates an Event with its ECompetitions
    </rdfs:comment>
    <owl:inverseOf rdf:resource="#isEventOf" /> 
    <rdfs:domain rdf:resource="#ECompetition" />
    <rdfs:range rdf:resource="#Event" />
    <rdfs:label xml:lang="en">hasEvent</rdfs:label>
    <rdfs:label xml:lang="fr">eventementDe</rdfs:label>
  </owl:ObjectProperty>
  
  <owl:ObjectProperty rdf:about="hasPoints">
    <rdfs:comment xml:lang="en">
      Number of points given for winning in any ESports competition
    </rdfs:comment>
    <rdfs:label xml:lang="en">has points</rdfs:label>
    <rdfs:label xml:lang="fr">tiens points</rdfs:label>
  </owl:ObjectProperty>
  
  <owl:Class rdf:about="ECompetition">
    <rdfs:comment xml:lang="en">
      A competition can be understood as a league of a specific game, the participants
  	compete making point across the events to have better position in the classification.
    </rdfs:comment>
    <rdfs:label xml:lang="en">ECompetition</rdfs:label>
    <rdfs:label xml:lang="fr">ECompetition</rdfs:label>
  </owl:Class>
  
  <owl:ObjectProperty rdf:about="isECompetitionOf">
    <rdfs:comment xml:lang="en">
      This property relates the ECompetition with the ESports
    </rdfs:comment>
    <owl:inverseOf rdf:resource="#hasECompetition" /> 
    <rdfs:domain rdf:resource="#ECompetition" />
    <rdfs:range rdf:resource="#ESport" />
    <rdfs:label xml:lang="en">isECompetitionOf</rdfs:label>
    <rdfs:label xml:lang="fr">ecompetitionDe</rdfs:label>
  </owl:ObjectProperty>
  
  <owl:ObjectProperty rdf:about="hasECompetition">
    <rdfs:comment xml:lang="en">
      This property relates an ESport with its ECompetitions
    </rdfs:comment>
    <owl:inverseOf rdf:resource="#isECompetitionOf" /> 
    <rdfs:domain rdf:resource="#ESport" />
    <rdfs:range rdf:resource="#ECompetition" />
    <rdfs:label xml:lang="en">hasECompetition</rdfs:label>
    <rdfs:label xml:lang="fr">competitionDe</rdfs:label>
  </owl:ObjectProperty>
  
  <owl:Class rdf:about="EDivision">
    <rdfs:comment xml:lang="en">
      In the ESports as in any other competion there are different proffesional levels
    </rdfs:comment>
    <rdfs:label xml:lang="en">E-Division</rdfs:label>
    <rdfs:label xml:lang="fr">E-Division</rdfs:label>
  </owl:Class>
  
  <owl:ObjectProperty rdf:about="isEDivisionOf">
    <rdfs:comment xml:lang="en">
      This property relates an E-division with Events, ECompetitions or ESports
    </rdfs:comment>
    <owl:inverseOf rdf:resource="#hasECompetition" /> 
    <rdfs:domain rdf:resource="#EDivision" />
    <rdfs:label xml:lang="en">isECompetitionOf</rdfs:label>
    <rdfs:label xml:lang="fr">divisionDe</rdfs:label>
  </owl:ObjectProperty>
  
  <owl:ObjectProperty rdf:about="hasEDivision">
    <rdfs:comment xml:lang="en">
      This property relates Events, ECompetitions or ESports with their EDivisions
    </rdfs:comment>
    <owl:inverseOf rdf:resource="#isEDivisionOf" /> 
    <rdfs:range rdf:resource="#EDivision" />
    <rdfs:label xml:lang="en">hasEDivision</rdfs:label>
    <rdfs:label xml:lang="fr">divisionDe</rdfs:label>
  </owl:ObjectProperty>
  
  <owl:Class rdf:about="ESession">
    <rdfs:comment xml:lang="en">
      An ESession is a set of events
    </rdfs:comment>
    <rdfs:label xml:lang="en">ESession</rdfs:label>
    <rdfs:label xml:lang="fr">ESession</rdfs:label>
  </owl:Class>
  
  <owl:ObjectProperty rdf:about="isESessionOf">
    <rdfs:comment xml:lang="en">
      This property relates an ESession with an ECompetition
  	ESports have the particularity that the events in different places might be related to the same session of the League.
    </rdfs:comment>
    <owl:inverseOf rdf:resource="#hasESession" /> 
    <rdfs:domain rdf:resource="#ESession" />
    <rdfs:range rdf:resource="#ECompetition" />
    <rdfs:label xml:lang="en">isECompetitionOf</rdfs:label>
    <rdfs:label xml:lang="fr">divisionDe</rdfs:label>
  </owl:ObjectProperty>
  
  <owl:ObjectProperty rdf:about="hasESession">
    <rdfs:comment xml:lang="en">
      This property relates an ECompetition with an ESession
  	ESports have the particularity that the events in different places might be related to the same session of the League.
    </rdfs:comment>
    <owl:inverseOf rdf:resource="#isEDivisionOf" /> 
    <rdfs:domain rdf:resource="#ECompetition" />
    <rdfs:range rdf:resource="#ESession" />
    <rdfs:label xml:lang="en">hasESession</rdfs:label>
    <rdfs:label xml:lang="fr">sessionDe</rdfs:label>
  </owl:ObjectProperty>
  
  <owl:Class rdf:about="EStage">
    <rdfs:comment xml:lang="en">
      Within a session there might be different rounds (i.e. a round of 16, a round of 8, quarter finals, semifinals, finals)
    </rdfs:comment>
    <owl:sameAs rdf:resource="#ERound" />
    <rdfs:label xml:lang="en">EStage</rdfs:label>
    <rdfs:label xml:lang="fr">EStage</rdfs:label>
  </owl:Class>
  
  <owl:Class rdf:about="ERound">
    <rdfs:comment xml:lang="en">
      Within a session there might be different stages (i.e. a stage of 16, a stage of 8, quarter finals, semifinals, finals)
    </rdfs:comment>
    <owl:sameAs rdf:resource="#EStage" />
    <rdfs:label xml:lang="en">ERound</rdfs:label>
    <rdfs:label xml:lang="fr">ERound</rdfs:label>
  </owl:Class>
  
  <owl:ObjectProperty rdf:about="isERoundOf">
    <rdfs:comment xml:lang="en">
      This property relates an ERound with an ESession
    </rdfs:comment>
    <owl:inverseOf rdf:resource="#hasERound" /> 
    <rdfs:domain rdf:resource="#ERound" />
    <rdfs:range rdf:resource="#ESession" />
    <rdfs:label xml:lang="en">isERoundOf</rdfs:label>
    <rdfs:label xml:lang="fr">tournéeDe</rdfs:label>
  </owl:ObjectProperty>
  
  <owl:ObjectProperty rdf:about="hasERound">
    <rdfs:comment xml:lang="en">
      This property relates an ESession with an ESRound
    </rdfs:comment>
    <owl:inverseOf rdf:resource="#isERoundOf" /> 
    <rdfs:domain rdf:resource="#ESession" />
    <rdfs:range rdf:resource="#ERound" />
    <rdfs:label xml:lang="en">hasERound</rdfs:label>
    <rdfs:label xml:lang="fr">tournéeDe</rdfs:label>
  </owl:ObjectProperty>
  
  <owl:Class rdf:about="EGroupCompetition">
    <rdfs:comment xml:lang="en">
      When there's a large number of teams, these are splitted into groups within the rounds. 
  	For instance the round of 16 can have A - F group competions to hold and to arrange all the
  	participant teams
    </rdfs:comment>
    <rdfs:label xml:lang="en">EGroupCompetition</rdfs:label>
    <rdfs:label xml:lang="fr">EGroupCompetition</rdfs:label>
  </owl:Class>
  
  <owl:ObjectProperty rdf:about="isEGroupCompetitionOf">
    <rdfs:comment xml:lang="en">
      This property relates an EGroupCompetition with an ERound
    </rdfs:comment>
    <owl:inverseOf rdf:resource="#hasEGroupCompetition" /> 
    <rdfs:domain rdf:resource="#EGroupCompetition" />
    <rdfs:range rdf:resource="#ERound" />
    <rdfs:label xml:lang="en">isEGroupCompetitionOf</rdfs:label>
    <rdfs:label xml:lang="fr">groupeDe</rdfs:label>
  </owl:ObjectProperty>
  
  <owl:ObjectProperty rdf:about="hasEGroupCompetition">
    <rdfs:comment xml:lang="en">
      This property relates an ERound with an EGroupCompetition
    </rdfs:comment>
    <owl:inverseOf rdf:resource="#isEGroupCompetitionOf" /> 
    <rdfs:domain rdf:resource="#ERound" />
    <rdfs:range rdf:resource="#EGroupCompetition" />
    <rdfs:label xml:lang="en">hasEGroupCompetition</rdfs:label>
    <rdfs:label xml:lang="fr">groupeDe</rdfs:label>
  </owl:ObjectProperty>
  
  <owl:Class rdf:about="EMatch">
    <rdfs:comment xml:lang="en">
      A match is a game between different teams or individual players
    </rdfs:comment>
    <rdfs:label xml:lang="en">EMatch</rdfs:label>
    <rdfs:label xml:lang="fr">EMatch</rdfs:label>
  </owl:Class>
  
  <owl:ObjectProperty rdf:about="isEMatchOf">
    <rdfs:comment xml:lang="en">
      This property relates an EMatch with an EGroupCompetition, an Event or an ERound
    </rdfs:comment>
    <owl:inverseOf rdf:resource="#hasEMatch" /> 
    <rdfs:domain rdf:resource="#EMatch" />
    <rdfs:label xml:lang="en">isEMatch</rdfs:label>
    <rdfs:label xml:lang="fr">matchDe</rdfs:label>
  </owl:ObjectProperty>
  
  <owl:ObjectProperty rdf:about="hasEMatch">
    <rdfs:comment xml:lang="en">
      This property relates an EGroupCompetition, an Event or an ERound with an EMatch
    </rdfs:comment>
    <owl:inverseOf rdf:resource="#isEMatchOf" /> 
    <rdfs:range rdf:resource="#EMatch" />
    <rdfs:label xml:lang="en">hasEMatch</rdfs:label>
    <rdfs:label xml:lang="fr">matchDe</rdfs:label>
  </owl:ObjectProperty>
  
  <owl:ObjectProperty rdf:about="previousECompetition">
    <rdfs:comment xml:lang="en">
      Sets the previous Event, ECompetition, EMatch, ...
    </rdfs:comment>
    <rdf:type rdf:resource="&owl;TransitiveProperty"/>
    <owl:inverseOf rdf:resource="#nextECompetition" />
    <rdfs:label xml:lang="en">previous competition</rdfs:label>
    <rdfs:label xml:lang="fr">anterieur competition</rdfs:label>
  </owl:ObjectProperty>
  
  <owl:ObjectProperty rdf:about="nextECompetition">
    <rdfs:comment xml:lang="en">
      Sets the previous Event, ECompetition, EMatch, ...
    </rdfs:comment>
    <rdf:type rdf:resource="&owl;TransitiveProperty"/>
    <owl:inverseOf rdf:resource="#previousECompetition" />
    <rdfs:label xml:lang="en">next e-competition</rdfs:label>
    <rdfs:label xml:lang="fr">suivant e-competition</rdfs:label>
  </owl:ObjectProperty>
  
  <owl:ObjectProperty rdf:about="multigameConsistsOf">
    <rdfs:comment xml:lang="en">
      Some of the ECompetition (Events, EMatches, ERounds, ...) may consists of different ESports (multigame)
    </rdfs:comment>
    <rdfs:range rdf:resource="#ESport" />
    <rdfs:label xml:lang="en">multigame ECompetition consists of</rdfs:label>
    <rdfs:label xml:lang="fr">competetion multijéu basé sur</rdfs:label>
  </owl:ObjectProperty>
  
  <owl:ObjectProperty rdf:about="hasDate">
    <rdfs:comment xml:lang="en">
      This property sets the date of any variety of sports event
    </rdfs:comment>
    <rdfs:subClassOf rdf:resource="&dc;date" />
    <owl:minCardinality rdf:datatype="&xsd;nonNegativeInteger">1</owl:minCardinality>
  </owl:ObjectProperty>
  
  <owl:Class rdf:about="EPlayer">
    <rdfs:comment xml:lang="en">
      A player is a person who play ESports individually or within a team
    </rdfs:comment>
    <rdfs:subClassOf rdf:resource="&foaf;Person" />
    <rdfs:label xml:lang="en">person</rdfs:label>
    <rdfs:label xml:lang="fr">personne</rdfs:label>
  </owl:Class>
  
  <owl:Class rdf:about="ETeam">
    <rdfs:comment xml:lang="en">
      Group of players which competes in ESports
    </rdfs:comment>
	<rdfs:subClassOf rdf:resource="&foaf;Group" />
    <rdfs:label xml:lang="en">team</rdfs:label>
    <rdfs:label xml:lang="fr">équipe</rdfs:label>
  </owl:Class>
  
  <!-- RDF DATA !-->
  
  <owl:AllDifferent>
    <owl:distinctMembers rdf:parseType="Collection">
      <VideoConsole rdf:about="#PS1" />
      <VideoConsole rdf:about="#PS2" />
	  <VideoConsole rdf:about="#PS3" />
	  <VideoConsole rdf:about="#PS4" />
	  <VideoConsole rdf:about="#XBox" />
	  <VideoConsole rdf:about="#PC" />
    </owl:distinctMembers>
  </owl:AllDifferent>
 
  <VideoGame rdf:ID="LeagueOfLegends">
	 <playInConsole rdf:resource="#PC" />
  </VideoGame>
  
  <VideoGame rdf:ID="FIFA">
	 <basedOn rdf:resource="#Football" />
	 <playInConsole rdf:resource="#PS2" />
	 <playInConsole rdf:resource="#PS3" />
	 <playInConsole rdf:resource="#PS4" />
	 <playInConsole rdf:resource="#XBox" />
	 <playInConsole rdf:resource="#PC" />
  </VideoGame>
  
  <VideoGame rdf:ID="PRO">
	 <basedOn rdf:resource="#Football" />
	 <playInConsole rdf:resource="#PS4" />
	 <playInConsole rdf:resource="#PC" />
  </VideoGame>
  
  <VideoGame rdf:ID="F1">
	 <basedOn rdf:resource="#Football" />
	 <playInConsole rdf:resource="#PS4" />
	 <playInConsole rdf:resource="#PC" />
  </VideoGame>
  
  <owl:AllDifferent>
    <owl:distinctMembers rdf:parseType="Collection">
      <sports:Sport rdf:about="#Football" />
      <sports:Sport rdf:about="#Chess" />
	  <sports:Sport rdf:about="#Racing" />
	  <sports:Sport rdf:about="#Fight" />
    </owl:distinctMembers>
  </owl:AllDifferent>
  
  <owl:AllDifferent>
    <owl:distinctMembers rdf:parseType="Collection">
      <ERound rdf:about="#QuarterFinals">
	    <hasName>Quarter Finals</hasName>
	  </ERound>
	  <ERound rdf:about="#SemiFinals">
	    <hasName>Semi Finals</hasName>
	  </ERound>
	  <ERound rdf:about="#Final" >
	    <hasName>Final</hasName>
	  </ERound>
    </owl:distinctMembers>
  </owl:AllDifferent>
  
  <ECompetition rdf:ID="EULCSSPRING">
    <hasName>2015 NA LCS Spring Split</hasName>
	<hasDescription>
	  The NA Spring Finals weekend kicks off with the battle for 
	  3rd place on Saturday, April 16. Then, we’ll switch over to 
	  the high-stakes match of the top two teams fighting to win the 
	  2016 NA LCS Spring Split on Sunday, April 17. The NA Spring 
	  Finals champion will also represent North America at the 2016
	  Mid-Season Invitational (MSI).
	</hasDescription>
	<isECompetitionOf rdf:resource="#eLeagueOfLegends" />
	<hasPoints rdf:datatype="http://www.w3.org/2001/XMLSchema#nonNegativeInteger">90</hasPoints>
	<hasEvent>
	  <Event rdf:ID="EULCSSPRINGPlayoffs">
	    <hasDate>2015-03-30</hasDate>
	    <geonames:locatedIn>
	      <geonames:Feature>
	        <geonames:name>Europe</geonames:name>
	      </geonames:Feature>
	    </geonames:locatedIn>
	  </Event>
	</hasEvent>
	<hasWeb>http://euw.lolesports.com/</hasWeb>
	<hasERound rdf:resource="#QuarterFinals" />
	<hasERound rdf:resource="#SemiFinals" />
	<hasERound rdf:resource="#Final" />
  </ECompetition>

  <ECompetition rdf:ID="EULCSSUMMER">
    <hasName>EU LCS Summer</hasName>
	<hasDescription>
	  The 2015 Season Championship Series is the third season of Europe's fully 
	  professional League of Legends league. In the playoffs six teams will compete 
	  in a single elimination bracket, with first and second place being seeded into 
	  the semifinals. The finals and third place matches are being held in the Hovet 
	  Arena in Stockholm, Sweden. The winner of the Summer Playoffs automatically 
	  qualifies for the 2015 Season World Championship as the number one seed from 
	  Europe.
	</hasDescription>
	<isECompetitionOf rdf:resource="#eLeagueOfLegends" />
	<hasPoints rdf:datatype="http://www.w3.org/2001/XMLSchema#nonNegativeInteger">50000</hasPoints>
	<hasEvent>
	  <Event rdf:ID="EULCSSUMMERPlayoffs">
	    <hasDate>2015-05-28</hasDate>
	    <geonames:locatedIn>
	      <geonames:Feature>
	        <geonames:name>Europe</geonames:name>
	      </geonames:Feature>
	    </geonames:locatedIn>
	  </Event>
	</hasEvent>
	<hasWeb>http://euw.lolesports.com/</hasWeb>
	<hasERound rdf:resource="#QuarterFinals" />
	<hasERound rdf:resource="#SemiFinals" />
	<hasERound rdf:resource="#Final" />
  </ECompetition>
  
  <ECompetition rdf:ID="EUNASUMMER">
    <hasName>2015 NA LCS Summer Split</hasName>
	<hasDescription>
	  In the event that multiple teams are tied in the standings at the conclusion 
	  of the Summer Split, then the team that gained the most points in the Summer 
	  Split will be considered the holder of the tiebreaker.
	</hasDescription>
	<isECompetitionOf rdf:resource="#eLeagueOfLegends" />
	<hasPoints rdf:datatype="http://www.w3.org/2001/XMLSchema#nonNegativeInteger">0</hasPoints>
	<hasEvent>
	  <Event rdf:ID="EUNASUMMERPlayoffs">
	    <hasDate>-05-30</hasDate>
	    <geonames:locatedIn>
	      <geonames:Feature>
	        <geonames:name>USA</geonames:name>
	      </geonames:Feature>
	    </geonames:locatedIn>
	  </Event>
	</hasEvent>
	<hasWeb>http://na.lolesports.com/</hasWeb>
	<hasERound rdf:resource="#QuarterFinals" />
	<hasERound rdf:resource="#SemiFinals" />
	<hasERound rdf:resource="#Final" />
  </ECompetition>
  
  <ECompetition rdf:ID="Azubu">
    <hasName>Azubu The Champions Summer 2012</hasName>
	<hasDescription>
	  Azubu Blaze, formerly named MiG Blaze, is one of two squads sponsored 
	  by German media group Azubu. They were added to Maximum impact Gaming's 
	  roster after MiG Frost, now Azubu Frost, won the OnGameNet LoL Invitational.
	</hasDescription>
	<isECompetitionOf rdf:resource="#eLeagueOfLegends" />
	<hasPoints rdf:datatype="http://www.w3.org/2001/XMLSchema#nonNegativeInteger">10000</hasPoints>
	<hasEvent>
	  <Event rdf:ID="Azubu">
	    <hasDate>2012-07-04</hasDate>
	    <geonames:locatedIn>
	      <geonames:Feature>
	        <geonames:name>South Corea</geonames:name>
	      </geonames:Feature>
	    </geonames:locatedIn>
	  </Event>
	</hasEvent>
	<hasWeb>http://www.ognlol.com/</hasWeb>
	<hasERound rdf:resource="#QuarterFinals" />
	<hasERound rdf:resource="#SemiFinals" />
	<hasERound rdf:resource="#Final" />
  </ECompetition>
  
  <ECompetition rdf:ID="EULCSSpringPromo">
    <hasName>2016 EU LCS Spring Promo</hasName>
	<hasDescription>
	  2 Challenger Teams are matched up with 8th and 9th place 
	  LCS teams, and the winners make it to Summer Split
	</hasDescription>
	<isECompetitionOf rdf:resource="#eLeagueOfLegends" />
	<hasPoints rdf:datatype="http://www.w3.org/2001/XMLSchema#nonNegativeInteger">50000</hasPoints>
	<hasEvent>
	  <Event rdf:ID="EULCSSpringPromo">
	    <hasDate>2016</hasDate>
	    <geonames:locatedIn>
	      <geonames:Feature>
	        <geonames:name>Europe</geonames:name>
	      </geonames:Feature>
	    </geonames:locatedIn>
	  </Event>
	</hasEvent>
	<hasWeb>http://www.riotgames.com/</hasWeb>
	<hasERound rdf:resource="#Final" />
  </ECompetition>
  
  <ECompetition rdf:ID="IEMSeasonIX">
    <hasName>IEM Season IX</hasName>
	<hasDescription>
	  The Intel Extreme Masters is ESL's flagship competition sponsored by Intel. 
	  IEM is a huge tournament spanning many months and individual competitions culminating in the 
	  Global Championships. While each year the games played changes, for Season IX, Starcraft 
	  2 will be played alongside League of Legends.
	</hasDescription>
	<isECompetitionOf rdf:resource="#eLeagueOfLegends" />
	<hasPoints rdf:datatype="http://www.w3.org/2001/XMLSchema#nonNegativeInteger">100000</hasPoints>
	<hasEvent>
	  <Event rdf:ID="IEMSeasonIX">
	    <hasDate>2015-03-12</hasDate>
	    <geonames:locatedIn>
	      <geonames:Feature>
	        <geonames:name>Europe</geonames:name>
	      </geonames:Feature>
	    </geonames:locatedIn>
	  </Event>
	</hasEvent>
	<hasWeb>http://intelextrememasters.com/</hasWeb>
	<hasERound rdf:resource="#Final" />
  </ECompetition>
  
  <ESport rdf:ID="eLeagueOfLegends">
    <hasName>League Of Legends</hasName>
    <derivedFrom rdf:resource="#LeagueOfLegends" />
	<hasCompetition rdf:resource="#WorldChampionship" />
    <hasCompetition rdf:resource="#WorldChampionship" />
	<hasCompetition rdf:resource="#EuropeanChampionship" />
	<hasCompetition rdf:resource="#FrenchChampionship" />
  </ESport>
  
  <ESport rdf:ID="eFIFA">
    <hasName>FIFA</hasName>
    <derivedFrom rdf:resource="#FIFA" />
    <hasCompetition rdf:resource="#WorldChampionship" />
  </ESport>
  
  <ESport rdf:ID="ePRO">
    <hasName>PRO</hasName>
	<derivedFrom rdf:resource="#PRO" />
	<hasCompetition rdf:resource="#WorldChampionship" />
	<hasCompetition rdf:resource="#EuropeanChampionship" />
	<hasCompetition rdf:resource="#FrenchChampionship" />
  </ESport>
  
  <ESport rdf:ID="eF1">
    <hasName>F1</hasName>
	<derivedFrom rdf:resource="#F1" />
	<hasCompetition rdf:resource="#WorldChampionship" />
  </ESport>
  
  <ETeam rdf:ID="&dbpedia;Fnatic">
	<hasName>Fnatic</hasName>
	<hasUri>http://dbpedia.org/resource/Fnatic</hasUri>
	<hasWeb>http://www.fnatic.com</hasWeb>
	<playInConsole rdf:resource="#PS2" />
	<hasWon rdf:resource="#EULCSSPRING" />
	<hasWon rdf:resource="#EULCSSUMMER" />
	<foaf:member>
	  <EPlayer rdf:ID="Gamsu">
  	    <foaf:geekcode>Gamsu</foaf:geekcode>
  	    <foaf:firstName>Yeong-Jin</foaf:firstName>
  	    <foaf:lastName>Noh</foaf:lastName>
  	    <memberOf rdf:resource="#Fnatic" />
      </EPlayer>
    </foaf:member>
	<foaf:member>
      <EPlayer rdf:ID="Noxiak">
  	    <foaf:geekcode>Noxiak</foaf:geekcode>
  	    <foaf:firstName>Felix</foaf:firstName>
  	    <foaf:lastName>Lewis</foaf:lastName>
  	    <memberOf rdf:resource="#Fnatic" />
      </EPlayer>
    </foaf:member>
	<foaf:member>
      <EPlayer rdf:ID="Spirit">
  	    <foaf:geekcode>Spirit</foaf:geekcode>
  	    <foaf:firstName>Lee</foaf:firstName>
  	    <foaf:lastName>Dayun</foaf:lastName>
  	    <memberOf rdf:resource="#Fnatic" />
      </EPlayer>
    </foaf:member>
	<foaf:member>
      <EPlayer rdf:ID="Febiven">
  	    <foaf:geekcode>Febiven</foaf:geekcode>
  	    <foaf:firstName>Fabian</foaf:firstName>
  	    <foaf:lastName>Diepstraten</foaf:lastName>
  	    <memberOf rdf:resource="#Fnatic" />
      </EPlayer>
    </foaf:member>
    <foaf:member>	
      <EPlayer rdf:ID="Rekkles">
  	    <foaf:geekcode>Rekkles</foaf:geekcode>
  	    <foaf:firstName>Martin</foaf:firstName>
  	    <foaf:lastName>Larsson</foaf:lastName>
  	    <memberOf rdf:resource="#Fnatic" />
      </EPlayer>
	</foaf:member>
  </ETeam>
  
  <ETeam rdf:ID="&dbpedia;Team_Liquid">
	<hasName>Team Liquid</hasName>
	<hasUri>http://dbpedia.org/resource/Team_Liquid</hasUri>
	<hasWeb>http://www.liquidlegends.net/</hasWeb>
	<hasWon rdf:resource="#EULCSSUMMER" />
	<foaf:member>
	  <EPlayer rdf:ID="Lourlo">
        <foaf:geekcode>Lourlo</foaf:geekcode>
        <foaf:firstName>Samson</foaf:firstName>
        <foaf:lastName>Jackson</foaf:lastName>
        <memberOf rdf:resource="#TeamLiquid" />
      </EPlayer>
	</foaf:member>
    <foaf:member>
	  <EPlayer rdf:ID="Dardoch">
		<foaf:geekcode>Dardoch</foaf:geekcode>
		<foaf:firstName>Joshua</foaf:firstName>
		<foaf:lastName>Hartnett</foaf:lastName>
		<memberOf rdf:resource="#TeamLiquid" />
	  </EPlayer>
	</foaf:member>
    <foaf:member>	
	  <EPlayer rdf:ID="FeniX">
		<foaf:geekcode>FeniX</foaf:geekcode>
		<foaf:firstName>Kim</foaf:firstName>
		<foaf:lastName>Jae-hoon</foaf:lastName>
		<memberOf rdf:resource="#TeamLiquid" />
	  </EPlayer>
	</foaf:member>
    <foaf:member>	
	  <EPlayer rdf:ID="Piglet">
		<foaf:geekcode>Piglet</foaf:geekcode>
		<foaf:firstName>Chae</foaf:firstName>
		<foaf:lastName>Gwang-jin</foaf:lastName>
		<memberOf rdf:resource="#TeamLiquid" />
	  </EPlayer>
	</foaf:member>
    <foaf:member>	
	  <EPlayer rdf:ID="Matt">
		<foaf:geekcode>Matt</foaf:geekcode>
		<foaf:firstName>Matt</foaf:firstName>
		<foaf:lastName>Elento</foaf:lastName>
		<memberOf rdf:resource="#TeamLiquid" />
	  </EPlayer>
	</foaf:member>
  </ETeam>
  
  <ETeam rdf:ID="&dbpedia;Natus_Vincere">
    <hasName>Natus Vincere</hasName>
	<hasUri>http://dbpedia.org/resource/Natus_Vincere</hasUri>
	<hasWon rdf:resource="#Azubu" />
    <hasWeb>http://navi-gaming.com/en</hasWeb>
    <foaf:member>
  	  <EPlayer rdf:ID="Jwaow">
	    <foaf:geekcode>Jwaow</foaf:geekcode>
	    <foaf:firstName>Jesper</foaf:firstName>
	    <foaf:lastName>Strandgren</foaf:lastName>
	    <memberOf rdf:resource="#NatusVincere" />
	  </EPlayer>
	</foaf:member>
	<foaf:member>   
	  <EPlayer rdf:ID="Amin">
	    <foaf:geekcode>Amin</foaf:geekcode>
	    <foaf:firstName>Amin</foaf:firstName>
	    <foaf:lastName>Mezher</foaf:lastName>
	    <memberOf rdf:resource="#NatusVincere" />
	  </EPlayer>
	</foaf:member>
	<foaf:member>
	  <EPlayer rdf:ID="SozPurefect">
	    <foaf:geekcode>SozPurefect</foaf:geekcode>
	    <foaf:firstName>Hicham</foaf:firstName>
	    <foaf:lastName>Tazrhini</foaf:lastName>
	    <memberOf rdf:resource="#NatusVincere" />
	  </EPlayer>
	</foaf:member>
	<foaf:member>
	  <EPlayer rdf:ID="EXORKK">
	    <foaf:geekcode>EXORKK</foaf:geekcode>
	    <foaf:firstName>Sébastien</foaf:firstName>
	    <foaf:lastName>Lamorte</foaf:lastName>
	    <memberOf rdf:resource="#NatusVincere" />
	  </EPlayer>		
    </foaf:member>
    <foaf:member>	
	  <EPlayer rdf:ID="MounTain">
	    <foaf:geekcode>MounTain</foaf:geekcode>
	    <foaf:firstName>Patrick</foaf:firstName>
	    <foaf:lastName>Dasberg</foaf:lastName>
	    <memberOf rdf:resource="#NatusVincere" />
	  </EPlayer>
    </foaf:member> 
    <foaf:member>	
	  <EPlayer rdf:ID="Czaru">
	    <foaf:geekcode>Czaru</foaf:geekcode>
	    <foaf:firstName>Krystian</foaf:firstName>
	    <foaf:lastName>Przybylski</foaf:lastName>
	    <memberOf rdf:resource="#NatusVincere" />
	  </EPlayer>
    </foaf:member>
  </ETeam>
  
  <ETeam rdf:ID="&dbpedia;SK_Gaming">
	<hasName>SKGaming</hasName>
	<hasUri>http://dbpedia.org/resource/SK_Gaming</hasUri>
	<hasWon rdf:resource="#IEMSeasonIX" />
	<hasWon rdf:resource="#EULCSSpringPromo" />
	<hasWeb>http://www.sk-gaming.com/</hasWeb>
	<foaf:member>
      <EPlayer rdf:ID="Morsu">
        <foaf:geekcode>Morsu</foaf:geekcode>
        <foaf:firstName>Bram</foaf:firstName>
        <foaf:lastName>Knol</foaf:lastName>
        <memberOf rdf:resource="#SKGaming" />
      </EPlayer>
    </foaf:member>
    <foaf:member>	
      <EPlayer rdf:ID="Dokgo">
        <foaf:geekcode>Dokgo</foaf:geekcode>
        <foaf:firstName>Kim</foaf:firstName>
        <foaf:lastName>Kyeong-tak</foaf:lastName>
        <memberOf rdf:resource="#SKGaming" />
      </EPlayer>
    </foaf:member>
    <foaf:member>	
      <EPlayer rdf:ID="SuNo">
        <foaf:geekcode>SuNo</foaf:geekcode>
        <foaf:firstName>An</foaf:firstName>
        <foaf:lastName>Sun-ho</foaf:lastName>
        <memberOf rdf:resource="#SKGaming" />
      </EPlayer>
    </foaf:member>
    <foaf:member>	
      <EPlayer rdf:ID="Vardags">
        <foaf:geekcode>Vardags</foaf:geekcode>
        <foaf:firstName>Pontus</foaf:firstName>
        <foaf:lastName>Dahlblom</foaf:lastName>
        <memberOf rdf:resource="#SKGaming" />
      </EPlayer>
    </foaf:member>
    <foaf:member>	
      <EPlayer rdf:ID="Unlimited">
        <foaf:geekcode>Unlimited</foaf:geekcode>
        <foaf:firstName>Petar</foaf:firstName>
        <foaf:lastName>Georgiev</foaf:lastName>
        <memberOf rdf:resource="#SKGaming" />
      </EPlayer>
	</foaf:member>
  </ETeam>
  
</rdf:RDF>